examples/sort/CompareMain1.v
@@ -25,13 +25,13 @@ Section PROOF.
   Section SKENV.
     Variable skenv: SkEnv.t.
 
-    Definition main_spec: fspec := mk_simple "Main" (X:=unit)
+    Definition main_spec: fspec := mk_simple (X:=unit)
                                              (fun _ => (
                                                   (fun _ o => ⌜o = ord_top⌝),
                                                   top2
                                              )).
 
-    Definition compare_spec:    fspec := compare_gen mycmp "Main".
+    Definition compare_spec:    fspec := compare_gen mycmp.
 
     Definition MainCmpsStb: list (gname * fspec) := [("compare", compare_spec)].
 
@@ -39,19 +39,22 @@ Section PROOF.
 
     Definition MainSbtb: list (gname * fspecbody) := [("main", mk_specbody main_spec (fun _ => APC;; trigger (Choose _))); ("compare", mk_specbody compare_spec (fun _ => trigger (Choose _)))].
 
-    Definition MainSem: ModSem.t := {|
-      ModSem.fnsems := List.map (fun '(fn, body) => (fn, fun_to_tgt (GlobalStb skenv) fn body)) MainSbtb;
-      ModSem.mn := "Main";
-      ModSem.initial_mr := ε;
-      ModSem.initial_st := tt↑;
-                                   |}
+    Definition SMainSem: SModSem.t := {|
+      SModSem.fnsems := MainSbtb;
+      SModSem.mn := "Main";
+      SModSem.initial_mr := ε;
+      SModSem.initial_st := tt↑;
+                                     |}
     .
+
   End SKENV.
 
-  Definition Main: Mod.t := {|
-    Mod.get_modsem := fun skenv => MainSem skenv;
-    Mod.sk := [("compare", Sk.Gfun)];
-  |}
+  Definition SMain: SMod.t := {|
+    SMod.get_modsem := fun _ => SMainSem;
+    SMod.sk := [("compare", Sk.Gfun)];
+                             |}
   .
+
+  Definition Main: Mod.t := (SMod.to_tgt GlobalStb) SMain.
 
 End PROOF.
